demo for addition 4-limb proof

proofs/src/proof_obligations_demo.v
@@ -2,7 +2,7 @@
 
 (* ** Setup *)
 Require Import ZArith.
-From mathcomp Require Import ssreflect ssrfun ssrbool eqtype.
+From mathcomp Require Import ssreflect ssrfun ssrbool seq eqtype.
 
 Set Implicit Arguments.
 Unset Strict Implicit.
@@ -10,141 +10,809 @@ Unset Printing Implicit Defensive.
 
 Open Local Scope Z_scope.
 
-(* ** Axiomatization of required operations *)
+(* ** Assignments and helper lemmas/tactics *)
 
-Section Reduce.
+Definition Assgn {T} (x y : T) := x = y.
 
-Definition w : Z := 64.
+Notation "x '<-' y" := (Assgn x y) (at level 70, no associativity).
 
-Variable R : Z.
+Lemma assgnK {T} {x y : T} : x <- y -> x = y.
+Proof. done. Qed.
 
-Variable rem_p : Z.
+Lemma assgnKl {T1 T2} {x1 y1 : T1} {x2 y2 : T2} : (x1,x2) <- (y1,y2) -> x1 = y1.
+Proof. by rewrite /Assgn; case. Qed.
 
-Variable Z_w : Type.
+Lemma assgnKr {T1 T2} {x1 y1 : T1} {x2 y2 : T2} : (x1,x2) <- (y1,y2) -> x2 = y2.
+Proof. by rewrite /Assgn; case. Qed.
 
-Variable Z_p : Type.
+Lemma assgnS {T1 T2} {x1 y1 : T1} {x2 y2 : T2} : (x1,x2) <- (y1,y2) -> x1 <- y1 /\ x2 <- y2.
+Proof. by rewrite /Assgn; case. Qed.
 
-Variable toZp : Z -> Z_p.
+Definition Ntag (n : nat) (P : Prop) := P.
 
-Variable z64 : Z_w.
+Lemma add_tag_imp (n : nat) (P : Prop):
+  P -> Ntag n P.
+Proof. by rewrite /Ntag. Qed.
 
-Variable of64 : Z_w -> Z.
+Lemma remove_tag_imp {n : nat} (P : Prop):
+  Ntag n P -> P.
+Proof. by rewrite /Ntag. Qed.
 
-Variable in64 : Z -> Z_w.
-
-Variable bound : Z -> Z -> Z -> bool.
-
-Variable ofbool : bool -> Z_w.
-
-Variable umul_h : Z_w -> Z_w -> Z_w.
-
-Variable umul_l : Z_w -> Z_w -> Z_w.
-
-Variable addc_cf : Z_w -> Z_w -> bool -> bool.
-
-(* hint that there is no overflow *)
-Variable addc_ncf : Z_w -> Z_w -> bool -> Z_w.
-
-Variable addc_r : Z_w -> Z_w -> bool -> Z_w.
-
-Variable cmul : bool -> Z_w -> Z_w.
-
-(* ** Definitions *)
-
-Definition rem_p64 := nosimpl in64 rem_p.
-
-Definition b2i (b : bool) : Z := if b then 1 else 0.
-
-Definition umul (x y : Z_w) := (umul_l x y, umul_h x y).
-
-Definition imul (x y : Z_w) := nosimpl umul_l x y.
-
-Definition add (x y : Z_w) : bool * Z_w :=
-  (addc_cf x y false, addc_r x y false).
-
-Definition addc (x y : Z_w) (cf : bool) : bool * Z_w :=
-  (addc_cf x y cf, addc_r x y cf).
-
-Definition add_ncf (x y : Z_w) : Z_w := addc_ncf x y false.
-
-Definition bound_u64 (x : Z) := bound 0 x (2^64 - 1).
-
-(* ** Rewriting rules  *)
-
-Lemma of64_addc_r (x y : Z_w) (cf : bool):
-  of64 (addc_r x y cf) = of64 x + of64 y + b2i cf - b2i (addc_cf x y cf)*R.
-Admitted.
-
-Lemma of64_addc_ncf (x y : Z_w) (cf : bool):
-  bound_u64 (of64 x + of64 y + b2i cf) ->
-  of64 (addc_ncf x y cf) = of64 x + of64 y + b2i cf.
-Admitted.
-
-Lemma of640: of64 z64 = 0. Admitted.
-
-Lemma of64_cmul (cf : bool):
-  of64 (cmul cf rem_p64) = b2i cf * rem_p. Admitted.
-
-(* ** Addition for 2 limbs  *)
-
-Definition add_2limb(x0 x1 y0 y1 : Z_w) : (Z_w * Z_w) := 
-  let (cf, z0) := add  x0 y0      in
-  let (cf, z1) := addc x1 y1 cf   in
-  let u        := cmul cf rem_p64 in
-  let (cf, z0) := add  z0 u       in
-  let (cf, z1) := addc z1 z64 cf  in
-  let u        := cmul cf rem_p64 in
-  let z0       := add_ncf z0 u    in
-  (z0,z1).
-
-Lemma corr_add_2limb (x0 x1 y0 y1 : Z_w):
-  rem_p = R*R ->
-  let r := add_2limb x0 x1 y0 y1 in
-  match r with
-  | (z0,z1) =>
-       (of64 z0) + (of64 z1)*R
-     - ((of64 x0) + (of64 x1)*R + (of64 y0) + (of64 y1)*R)
-     = 0
+Ltac add_tag_rec N :=
+  match reverse goal with
+  | [ H : _ <- _  |- _ ] =>
+    let NN := constr:(S N) in
+    apply (add_tag_imp N) in H; add_tag_rec NN
+  | _ => idtac
   end.
+
+Ltac add_tag :=
+  let Z := constr:(0%nat) in
+  add_tag_rec Z.
+
+Ltac remove_tag :=
+  match goal with
+  | [ H : Ntag ?n _ |- _ ] =>
+    apply (@remove_tag_imp n) in H; remove_tag
+  | _ => idtac
+  end.
+
+Ltac contains_var T V :=
+  match T with
+  | context[V] => idtac
+  | _          => fail 1
+  end.
+
+Ltac is_lt N1 N2 :=
+  let C := eval compute in (N1 <? N2)%nat in
+  match C with
+  | false => fail
+  | true  => idtac
+  end.
+
+Ltac swap_hyps N1 N2 H1 H2 T V :=
+  (* H1 uses T containing V, H2 defines V => swap *)
+  is_lt N1 N2;
+  contains_var T V;
+  move: H2 H1 => H1 H2.
+
+Ltac swap_def_before_use :=
+  match goal with
+  | [ H1 : Ntag ?N1 (_ <- ?T), H2 : Ntag ?N2 (?D <- _) |- _ ] =>
+    match D with
+    | ?V     => is_var V; swap_hyps N1 N2 H1 H2 T V
+    | (?V,_) => is_var V; swap_hyps N1 N2 H1 H2 T V
+    | (_,?V) => is_var V; swap_hyps N1 N2 H1 H2 T V
+    end
+  end.
+
+Ltac push_defs :=
+  repeat match goal with
+         | [ H : _ <- _ |- _ ] => move: H
+         end.
+
+Ltac pop_defs :=
+  let L_ignore := fresh "L" in 
+  repeat match goal with
+        | [ _ : _ |- ?x <- ?y -> _] =>
+          let L1 := fresh "L" in move => L1
+         end.
+
+Ltac sort_defs :=
+  repeat try (add_tag; swap_def_before_use; remove_tag);
+  push_defs;
+  pop_defs.
+
+Ltac is_bool_const C :=
+  match C with
+  | true  => idtac
+  | false => idtac
+  |_      => fail
+  end.
+
+Ltac is_cmp_b O :=
+  match O with
+  | Z.leb => idtac
+  | Z.ltb => idtac
+  | _     => fail
+  end.
+
+Ltac trans_cmp_b_sym :=
+  repeat match goal with
+         | [ H : ?C = (?O _ _) |- _ ] =>
+           is_bool_const C; is_cmp_b O; apply Logic.eq_sym in H
+         | [ _ : _ |- ?C = (?O _ _) ] =>
+           is_bool_const C; is_cmp_b O; apply Logic.eq_sym
+         end.
+
+Ltac trans_cmp_b_simp :=
+  first [ rewrite Z.leb_gt | rewrite Z.leb_le | rewrite Z.ltb_ge | rewrite Z.ltb_lt ].
+
+Ltac trans_cmp_b :=
+  trans_cmp_b_sym;
+  repeat match goal with
+         | [ H : ( _ <=? _) = _ |- _ ] => move: H; trans_cmp_b_simp => H
+         | [ _ : _ |- ( _ <=? _) = _ ] => trans_cmp_b_simp
+         end.
+
+(* ** Word sizes and general lemmas *)
+
+Definition b2i (b : bool) := if b then 1 else 0.
+
+Notation "b ':%Z'"  := (b2i b) (at level 2, left associativity, format "b ':%Z'").
+
+Notation p64  := (locked (2^64)).
+Notation p128 := (p64*p64).
+Notation p192 := (p128*p64).
+Notation p256 := (p192*p64).
+Search positive nat.
+Notation pow n := (p64^(Z.of_nat n)).
+
+Lemma Z_pow_pos_gt0 (n : nat) : 0 < 2 ^ (Z.of_nat n).
 Proof.
-  move=> rem_p_R.
-  rewrite /= !(of64_addc_r, of64_addc_ncf, of640, of64_cmul, rem_p_R) /=.
-  (* ring takes care of the equality *)
-  ring.
-  (* but we still have to prove that whenever we ignore the carry bit, there
-     is no overflow *)
-  admit.
+elim n; first done.
+move=> {n} n H1. rewrite Nat2Z.inj_succ Z.pow_succ_r; last apply Nat2Z.is_nonneg.
+rewrite (_: 0 = 2 * 0); last done.
+by apply Zmult_lt_compat_l.
+Qed.
+
+Lemma pow_pos (n : nat) : 0 < pow n.
+Proof.
+elim n; first done.
+move => {n} n Hpos. rewrite Nat2Z.inj_succ Z.pow_succ_r; last apply Nat2Z.is_nonneg.
+rewrite (_: 0 = p64 * 0); last ring.
+apply Zmult_lt_compat_l; last done.
+rewrite (_: 64 = Z.of_nat 64); last done.
+by rewrite -lock; apply Z_pow_pos_gt0.
+Qed.
+
+Lemma Z_le_leq_succ (x y : Z): x < y <-> x <= y - 1.
+Proof.
+symmetry. rewrite {2}(_: y = Z.succ (y - 1)); last ring.
+split.
++ by apply Zle_lt_succ.
++ by move=> H; apply Zlt_succ_le in H.
+Qed.
+
+Lemma pow_ge0 (n : nat): 0 <= pow n.
+Proof. apply Z.lt_le_incl. apply pow_pos. Qed.
+
+Lemma p64_ge0: 0 <= p64.
+Proof.
+apply Z.lt_le_incl. rewrite -(Z.pow_1_r p64) (_ : 1 = Z.of_nat 1); last done.
+by apply pow_pos.
+Qed.
+
+Lemma Zeq_eq0 (x y : Z): 0 = x - y -> x = y.
+Proof. by rewrite -Zeq_plus_swap; move => <-. Qed.
+
+(* ** adc *)
+
+Definition adc_cf (n : nat) (u v : Z) (b : bool) : bool := (pow n) <=? (u + v) + b:%Z.
+Definition oflow  (n : nat) (u v : Z) (b : bool) : Z  := (adc_cf n u v b):%Z * (pow n).
+Definition adc_v  (n : nat) (u v : Z) (b : bool) : Z  := ((u + v) + b:%Z) - oflow n u v b.
+Notation adc n u v b := (adc_cf n u v b, adc_v n u v b).
+
+Lemma b2i_false: false:%Z = 0. Proof. done. Qed.
+Lemma b2i_true: true:%Z = 1. Proof. done. Qed.
+
+Definition is_u64 (n : Z) := (0 <=? n) && (n <? p64).
+
+Lemma is_u64K (n : Z): is_true (is_u64 n) <-> ( (0 <= n) /\ (n < p64)).
+Proof.
+rewrite /is_u64. split.
++ case/andP. rewrite /is_true Z.leb_le Z.ltb_lt. done.
++ case => H1 H2. apply/andP. rewrite /is_true Z.leb_le Z.ltb_lt. done.
+Qed.
+
+Lemma adc1_cf_0 (n : Z) :
+  is_u64 n -> adc_cf 1 n 0 false = false.
+Proof.
+rewrite is_u64K /adc_v /oflow /adc_cf b2i_false !Z.add_0_r Z.pow_1_r.
+move=> [h1 h2]. rewrite Z.leb_nle.
+apply Zgt_not_le. by apply Z.lt_gt.
+Qed.
+
+Lemma adc1_v_0 (n : Z) :
+  is_u64 n -> adc_v 1 n 0 false = n.
+Proof.
+move=> Hb. rewrite /adc_v /oflow adc1_cf_0 //=. ring.
+Qed.
+
+(* ** ds2i: list of digits to integer *)
+
+Fixpoint ds2i (ds : seq Z) :=
+  match ds with
+  | [::]  => 0
+  | d::ds => pow (length ds)*d + ds2i ds
+  end.
+
+Notation "[ ::i x0 ]" := (ds2i x0) (at level 0, format "[ ::i  x0 ]").
+
+Notation "[ :i x0 ]" := (ds2i [:: x0]) (at level 0, format "[ :i  x0 ]").
+
+Notation "[ :i x & s ]" := (ds2i (x :: s)) (at level 0, only parsing).
+
+Notation "[ :i x0 , x1 , .. , xn & s ]" := (ds2i (x0 :: x1 :: .. (xn :: s) ..))
+  (at level 0, format
+  "'[hv' [ :i '['  x0 , '/'  x1 , '/'  .. , '/'  xn ']' '/ '  &  s ] ']'").
+
+Notation "[ :i x0 ; x1 ; .. ; xn ]" := (ds2i (x0 :: x1 :: .. [:: xn] ..))
+  (at level 0, format "[ :i '['  x0 ; '/'  x1 ; '/'  .. ; '/'  xn ']' ]").
+
+Lemma ds2i_cons (x : Z) (xs : seq Z) : ds2i [:: x & xs] = pow (length xs)*x + ds2i xs.
+Proof. by rewrite //=. Qed.
+
+Lemma ds2i_0 (ds : seq Z) :
+  all (fun d => Z.eqb d 0) ds ->  ds2i ds = 0.
+Proof.
+elim ds; first done.
+move=> {ds} d ds Hind Hz. rewrite ds2i_cons.
+rewrite //= in Hz. move/andP: Hz => [].
+rewrite {1}/is_true Z.eqb_eq => -> Hall. rewrite Z.mul_0_r Z.add_0_l.
+by apply Hind.
+Qed.
+
+Lemma ds2i_nneg (ds : seq Z):
+  all (fun d => is_u64 d) ds ->
+  0 <= [::i ds].
+Proof.
+elim ds; first done.
+move=> {ds} d ds Hind. move/andP => [] Hd Hds.
+rewrite ds2i_cons.
+rewrite (_ : 0 = 0 + 0); last ring.
+apply (Z.add_le_mono).
+apply (Z.mul_nonneg_nonneg). apply pow_ge0. move/is_u64K : Hd => [] H1 H2. done.
+apply (Hind Hds).
+Qed.
+
+Lemma ds2i_bounded_lt (n : nat) (ds : seq Z):
+  length ds = n ->
+  all (fun d => is_u64 d) ds ->
+  [::i ds] < pow n.
+Proof.
+move: ds.
+elim n.
++  move=> [] //=.
++ move=> {n} n //= Hind ds //=.
+  case ds; first done. move=> {ds} d ds Hlen Hall.
+  rewrite //= in Hall. move/andP: Hall => [] His Hall.  
+  rewrite //= in Hlen. move: Hlen => [] Hlen.
+  move: (Hind ds Hlen Hall). rewrite ds2i_cons Hlen !Z.pow_pos_fold Zpos_P_of_succ_nat.
+  rewrite Z.pow_succ_r; last apply Nat2Z.is_nonneg.
+  move=> Hlt.
+  have H3: pow n * d + [::i ds] < pow n * d + pow n.
+  + apply Z.add_le_lt_mono; [ apply Z.eq_le_incl; ring | done].
+  apply (Z.lt_le_trans _ _ _ H3).
+  move: His.
+  rewrite is_u64K. case.
+  move=> G1 G2. rewrite (_: p64 = Z.succ (p64 - 1)) in G2; last ring.
+  move: (Zlt_succ_le _ _ G2) => G3.
+  rewrite (_: pow n * d + pow n = (d + 1) * pow n); last ring.
+  apply Z.mul_le_mono_pos_r. apply pow_pos.
+  rewrite (_: p64 = p64 - 1 + 1); last ring.
+  by apply Z.add_le_mono_r.
+Qed.
+
+Lemma ds2i_bounded_le (n : nat) (ds : seq Z):
+  length ds = n ->
+  all (fun d => is_u64 d) ds ->
+  [::i ds] <= pow n - 1.
+Proof.
+move=> H1 H2. apply Zlt_succ_le. ring_simplify.
+by apply ds2i_bounded_lt.
+Qed.
+
+(* ** adc with 0 argument *)
+
+Lemma adc_cf_0 (n : nat) (ds1 ds2 : seq Z):
+  length ds1 = n ->
+  all (fun d => is_u64 d) ds1 ->
+  all (fun d => Z.eqb d 0) ds2 ->
+  adc_cf n [::i ds1] [::i ds2] false = false.
+Proof.
+move=> Hlen Hall1 Hall2. rewrite (ds2i_0 Hall2).
+by rewrite /adc_cf b2i_false !Z.add_0_r Z.leb_gt; apply ds2i_bounded_lt.
+Qed.
+
+Lemma adc_v_0 (n : nat) (ds1 ds2 : seq Z):
+  length ds1 = n ->
+  all (fun d => is_u64 d) ds1 ->
+  all (fun d => Z.eqb d 0) ds2 ->
+  adc_v n [::i ds1] [::i ds2] false = [::i ds1].
+Proof.
+move=> Hlen Hall1 Hall2.
+rewrite /adc_v /oflow b2i_false !Z.add_0_r adc_cf_0 => //=.
+by rewrite (ds2i_0 Hall2); ring.
+Qed.
+
+(* ** Ltac *)
+
+Ltac band_auto :=
+  rewrite //=;
+  repeat
+    match goal with
+    | [ |- is_true (is_u64 _) ] => exact
+    | [ |- is_true (_ && _)   ] => apply/andP
+    | [ |- _ /\ _              ] => split
+    | [ |- is_true true       ] => done
+    end.
+
+Ltac rw_lez :=
+  match goal with
+  | [ H1 : context[adc_cf _ _ _ false] |- _ ] => rewrite adc1_cf_0 in H1; last done
+  | [ H1 : context[adc_v _ _ _ false] |- _  ] => rewrite adc1_v_0 in H1; last done
+  | [ H1 : context[adc_cf _ _ _ false] |- _ ] =>
+    rewrite adc_cf_0 in H1; [ idtac | done | band_auto | done ]
+  | [ H1 : context[adc_v _ _ _ false] |- _ ] =>
+    rewrite adc_v_0 in H1; [ idtac | done | band_auto | done ]
+  end.
+
+Ltac prop_false :=
+  match goal with
+  | [ H1 : ?x <- ?c        , H2 : context[?x] |- _ ] =>
+    is_bool_const c; is_var x; rewrite (assgnK H1) in H2
+  | [ H1 : (?x,_) <- (?c,_), H2 : context[?x] |- _ ] =>
+    is_bool_const c; is_var x; rewrite (assgnKl H1) in H2
+  | [ H1 : ?x <- 38 , H2   : _ |- _ ] => rewrite (assgnK H1) in H2
+  | [ H1 : ?x <- 0 , H2    : _ |- _ ] => rewrite (assgnK H1) in H2
+  end.
+
+Ltac prop_var_ctxt :=
+  match goal with
+  | [ H1 : ?x = ?y, H2 : is_u64 _ |- _ ] => fail 1
+  | [ H1 : ?x = ?y, H2 : context[?x] |- _ ] => is_var y; rewrite H1 in H2
+  end.
+
+Ltac simp_adc_v :=
+  match goal with
+  | [ H1 : ?x = adc_v _ _ _ ?cf |- _ ] =>
+      rewrite /adc_v /oflow in H1
+  end.
+
+Ltac simp_cf :=
+  match goal with
+  | [ H1 : ?x = _ + _ + _ - (b2i ?cf) * _ , H2 : _ = ?cf |- _ ] =>
+      rewrite -H2 in H1
+  | [ H1 : ?x = _ + _ - (b2i ?cf) * _ , H2 : _ = ?cf |- _ ] =>
+      rewrite -H2 in H1
+  end.
+
+Ltac prop_var_goal :=
+  match goal with
+  | [ H1 : ?x <- ?y    |- _ ] => is_var y; rewrite (assgnK H1)
+  | [ H1 : ?x <- ?c    |- _ ] => is_bool_const c; is_var x; rewrite (assgnK H1)
+  | [ H1 : (?x,_) <- (?c,_) |- _ ] => is_bool_const c; is_var x; rewrite (assgnKl H1)
+  | [ H1 : (_,?x) <- (_,?y) |- _ ] => is_var y; is_var x; rewrite (assgnKr H1)
+  | [ _ : _ |- _ ]           =>
+    first [ rewrite b2i_true | rewrite b2i_false | rewrite Z.add_0_r ]
+  | [ H1 : ?x = _     |- _ ] =>
+    first [ rewrite b2i_true in H1 | rewrite b2i_false in H1 | rewrite Z.add_0_r in H1 ]
+  end.
+
+Ltac prop_var_goal_all :=
+  match goal with
+  | [ H1 : ?x = _ |- context[?x] ] => rewrite H1
+  end.
+
+Ltac prop_0 :=
+  match goal with
+  | [ H1 : ?x = 0, H2 : _ |- _ ] => rewrite H1 in H2
+  end.
+
+Ltac simp_false :=
+  match goal with
+  | [ H : context[false:%Z] |- _ ] => rewrite b2i_false ?Z.add_0_r in H
+  end.
+
+Ltac simp_0 :=
+  match goal with
+  | [ H : _ |- _ ]  =>
+    first [ rewrite Z.mul_0_l in H | rewrite Z.mul_1_l in H
+          | rewrite Z.pow_1_r in H | rewrite Z.sub_0_r in H ]
+  | [ _ : _ |- _ ]  => rewrite Z.mul_0_l ?Z.sub_0_r ?Z.add_0_r
+  end.
+
+Ltac simp :=
+  repeat first [ rw_lez | prop_false | prop_0 | prop_var_ctxt | prop_var_goal
+               | simp_false | simp_0 | simp_adc_v | simp_cf
+               | rewrite Z.pow_1_r | rewrite Z.pow_0_r
+               | rewrite Z.mul_1_l | rewrite Z.mul_1_r ].
+
+Ltac not_adc t :=
+  match t with
+  | adc_cf _ _ _ _ => fail 1
+  | _              => idtac
+  end.
+
+Ltac inst_goal :=
+  repeat match goal with
+         | [ H : ?x = ?y |- context[?x] ] => is_var x; not_adc y; rewrite H
+         end.
+
+Ltac inst_goal_flag :=
+  repeat match goal with
+         | [ H : ?x = ?y |- context[?x] ] => is_var x; rewrite H
+         end.
+
+(* ** Combining adc in carry chains *)
+
+Lemma combine_chain1_cf (x0 y0 x1 y1 t0 t1 : Z) (cf0 cf1 cf2 :bool)
+  (B_x0: is_u64 x0)
+  (B_x1: is_u64 x1)
+  (B_y0: is_u64 y0)
+  (B_y1: is_u64 y1) :
+  (cf1,t0) <- adc 1 x0 y0 cf0 ->
+  (cf2,t1) <- adc 1 x1 y1 cf1 ->
+  cf2      <- adc_cf 2 [:i x1; x0] [:i y1; y0] cf0.
+Proof.
+move/assgnS => [] L0 L1. move/assgnS => [] L2 L3 {L3} {L1}.
+push_defs. rewrite /adc_cf /Assgn. unfold ds2i. unfold length. simp.
+have Hsucc : forall i, i = Z.succ (i - 1); first (move=> i; ring).
+have Hle: forall i, is_u64 i -> i <= p64 - 1.
++ move=> i. move/is_u64K => [] G1 G2.
+  rewrite (Hsucc p64) in G2.
+  by apply Zlt_succ_le in G2.
+have Hge: forall i, is_u64 i -> 0 <= i.
++ by move=> i; move/is_u64K => [] G1 G2.
+rewrite Z.pow_2_r.
+case cf2; last first.
++ case cf1; last first.
+  + move=> H1 H2. simp. trans_cmp_b.
+    rewrite (_:   p64 * x1 + x0 + (p64 * y1 + y0) + cf0:%Z
+                = p64 * (x1 + y1) + (x0 + y0 + cf0:%Z)); last ring.
+    move: H1 H2; rewrite !Z_le_leq_succ => H1 H2.
+    apply (Z.le_trans _ (p64 * (p64 - 1) + (p64 - 1))).
+    + apply (Z.add_le_mono); last done.
+      apply (Zmult_le_compat_l _ _ _ H2 p64_ge0).
+    rewrite (_ : p64 * (p64 - 1) + (p64 - 1) = (p64 * p64) - 1); last ring.
+    by apply Z.eq_le_incl.
+  + move=> H1 H2. simp. trans_cmp_b.
+    move: H1 H2; rewrite !Z_le_leq_succ => H1 H2.    
+    rewrite (_:   p64 * x1 + x0 + (p64 * y1 + y0) + cf0:%Z
+                = p64 * (x1 + y1) + (x0 + y0 + cf0:%Z)); last ring.
+    apply (Z.le_trans _ (p64 * (p64 - 2) + ((p64 - 1) + (p64 - 1) + 1))).
+    apply (Z.add_le_mono).
+    + apply (Zmult_le_compat_l _ _ _); last apply p64_ge0.
+      by apply (Zplus_le_reg_r _ _ 1); rewrite (_: p64 - 2 + 1 = p64 -1); last ring.
+    + apply (Z.add_le_mono); last by case cf0.
+      apply (Z.add_le_mono _ _ _ _ (Hle _ B_x0) (Hle _ B_y0)).
+    + by rewrite (_ :   p64 * (p64 - 2) + (p64 - 1 + (p64 - 1) + 1)
+                      = p64 * p64 - 1); [ apply Z.eq_le_incl | ring ].
++ case cf1.
+  + move=> H1 H2. simp. trans_cmp_b.
+    rewrite (_:   p64 * x1 + x0 + (p64 * y1 + y0) + cf0:%Z
+                = p64*(x1 + y1) + (x0 + y0 + cf0:%Z)); last ring.
+    rewrite (_ : p128 = p64*(p64 - 1) + p64); last ring.
+    apply (Z.add_le_mono); last done.
+    apply (Zmult_le_compat_l); last apply p64_ge0.
+    by apply (Zplus_le_reg_r _ _ 1); ring_simplify.
+  + move=> G H {G}. simp. trans_cmp_b.
+    rewrite (_ :   p64 * x1 + x0 + (p64 * y1 + y0) + cf0:%Z
+                 = p64 * (x1 + y1) + (x0 + y0 + cf0:%Z)); last ring.
+    rewrite (_ : p128 = p128 + (0 + 0 + 0)); last ring.
+    apply (Z.add_le_mono).
+    + by apply (Zmult_le_compat_l); last apply p64_ge0.
+    apply (Z.add_le_mono).
+    + by apply (Z.add_le_mono _ _ _ _ (Hge _ B_x0) (Hge _ B_y0)).
+    by case cf0.
+Qed.
+
+Lemma combine_chainN_cf (n : nat) (xn yn tn : seq Z) (xsn ysn tsn : Z) (cf0 cfn cfsn :bool) :
+  length xn = n ->
+  length yn = n ->
+  all (fun d => is_u64 d) xn ->
+  all (fun d => is_u64 d) yn ->
+  (cfn,[::i tn]) <- adc n [::i xn] [::i yn] cf0 ->
+  (cfsn,tsn)     <- adc 1 xsn ysn cfn ->
+  cfsn           <- adc_cf (S n) [:i xsn & xn] [:i ysn & yn] cf0.
+Proof.
+move=> Hlen_x Hlen_y Hall_x Hall_y.
+move/assgnS => [] L0 L1. move/assgnS => [] L2 L3 {L3} {L1}.
+push_defs. rewrite /adc_cf /Assgn. rewrite !ds2i_cons Hlen_x Hlen_y.
+have Hsucc : forall i, i = Z.succ (i - 1); first (move=> i; ring).
+have Hle: forall i, is_u64 i -> i <= p64 - 1.
++ move=> i. move/is_u64K => [] G1 G2.
+  rewrite (Hsucc p64) in G2.
+  by apply Zlt_succ_le in G2.
+have Hge: forall i, is_u64 i -> 0 <= i.
++ by move=> i; move/is_u64K => [] G1 G2.
+rewrite Z.pow_1_r.
+move=> H1 H2. rewrite !Nat2Z.inj_succ !Z.pow_succ_r; last apply Zle_0_nat.
+move: H1 H2. case cfsn; last first.
++ case cfn; last first.
+  + move=> H1 H2. simp. trans_cmp_b.
+    rewrite (_:   pow n * xsn + [::i xn] + (pow n * ysn + [::i yn]) + cf0:%Z 
+                = pow n * (xsn + ysn) + ([::i xn] + [::i yn] + cf0:%Z)); last ring.
+    move: H1 H2; rewrite !Z_le_leq_succ => H1 H2.
+    apply (Z.le_trans _ (pow n * (p64 - 1) + (pow n - 1))).
+    + apply (Z.add_le_mono); last done.
+      apply (Zmult_le_compat_l _ _ _ H2); first apply (pow_ge0).
+    rewrite (_ : pow n * (p64 - 1) + (pow n - 1) = (p64 * pow n) - 1); last ring.
+    by apply Z.eq_le_incl.
+  + move=> H1 H2. simp. trans_cmp_b.
+    move: H1 H2; rewrite !Z_le_leq_succ => H1 H2.    
+    rewrite (_:   pow n * xsn + [::i xn] + (pow n * ysn + [::i yn]) + cf0:%Z
+                = pow n * (xsn + ysn) + ([::i xn] + [::i yn] + cf0:%Z)); last ring.
+    apply (Z.le_trans _ (pow n * (p64 - 2) + ((pow n - 1) + (pow n - 1) + 1))).
+    apply (Z.add_le_mono).
+    + apply (Zmult_le_compat_l _ _ _); last apply pow_ge0.
+      by apply (Zplus_le_reg_r _ _ 1); rewrite (_: p64 - 2 + 1 = p64 -1); last ring.
+    + apply (Z.add_le_mono); last by case cf0.
+      apply (Z.add_le_mono _ _ _ _).
+      + by apply ds2i_bounded_le.
+      + by apply ds2i_bounded_le.      
+    + by rewrite (_ :   pow n * (p64 - 2) + (pow n - 1 + (pow n - 1) + 1)
+                      = p64 * pow n - 1); [ apply Z.eq_le_incl | ring ].
++ case cfn.
+  + move=> H1 H2. simp. trans_cmp_b.
+    rewrite (_:   pow n * xsn + [::i xn] + (pow n * ysn + [::i yn]) + cf0:%Z
+                = pow n * (xsn + ysn) + ([::i xn] + [::i yn] + cf0:%Z)); last ring.
+    rewrite (_ : p64*pow n = pow n*(p64 - 1) + pow n); last ring.
+    apply (Z.add_le_mono); last done.
+    apply (Zmult_le_compat_l); last (apply pow_ge0).
+    by apply (Zplus_le_reg_r _ _ 1); ring_simplify.
+  + move=> G H {G}. simp. trans_cmp_b.
+    rewrite (_ :   pow n * xsn + [::i xn] + (pow n * ysn + [::i yn]) + cf0:%Z
+                 = pow n * (xsn + ysn) + ([::i xn] + [::i yn] + cf0:%Z)); last ring.
+    rewrite (_ : p64 * pow n = pow n * p64 + (0 + 0 + 0)); last ring.
+    apply (Z.add_le_mono).
+    + by apply (Zmult_le_compat_l); last apply pow_ge0.
+    apply (Z.add_le_mono).
+    + apply (Z.add_le_mono _ _ _ _). apply (ds2i_nneg Hall_x). apply (ds2i_nneg Hall_y).
+    by case cf0.
+Qed.
+
+Lemma combine_chain1_v (x0 y0 x1 y1 t0 t1 : Z) (cf0 cf1 cf2 :bool)
+  (B_x0: is_u64 x0)
+  (B_x1: is_u64 x1)
+  (B_y0: is_u64 y0)
+  (B_y1: is_u64 y1) : 
+  (cf1,t0)    <- adc 1 x0 y0 cf0 ->
+  (cf2,t1)    <- adc 1 x1 y1 cf1 ->
+  [:i t1; t0] <- adc_v 2 [:i x1; x0] [:i y1; y0] cf0.
+Proof.
+move=> L0 L1.
+move: (combine_chain1_cf B_x0 B_x1 B_y0 B_y1 L0 L1) => H.
+move: L0 L1.
+move/assgnS => [] L0 L1. move/assgnS => [] L2 L3.
+rewrite L1 L3 L0 /adc_v /oflow /Assgn. unfold ds2i. unfold length. simp.
+apply Zeq_eq0.
+ring_simplify. rewrite {2}(_ : 2 = Z.of_nat 2); last done.
+unfold ds2i in H. unfold length in H.
+rewrite !Z.pow_1_r !Z.pow_0_r !Z.mul_1_l !Z.add_0_r in H.
+rewrite -H. move : L2. rewrite L0 => L2. rewrite -L2.
+ring.
+Qed.
+
+Lemma combine_chain1 (x0 y0 x1 y1 t0 t1 : Z) (cf0 cf1 cf2 :bool)
+  (B_x0: is_u64 x0)
+  (B_x1: is_u64 x1)
+  (B_y0: is_u64 y0)
+  (B_y1: is_u64 y1) : 
+  (cf1,t0)          <- adc 1 x0 y0 cf0 ->
+  (cf2,t1)          <- adc 1 x1 y1 cf1 ->
+  (cf2,[:i t1; t0]) <- adc 2 [:i x1; x0] [:i y1; y0] cf0.
+Proof.
+move=> H1 H2. congr pair.
++ by apply (combine_chain1_cf B_x0 B_x1 B_y0 B_y1 H1 H2).
++ by apply (combine_chain1_v B_x0 B_x1 B_y0 B_y1 H1 H2).
+Qed.
+
+Lemma combine_chainN_v (n : nat) (xn yn tn : seq Z) (xsn ysn tsn : Z) (cf0 cfn cfsn :bool) :
+  length xn = n ->
+  length yn = n ->
+  length tn = n -> 
+  all (fun d => is_u64 d) xn ->
+  all (fun d => is_u64 d) yn ->
+  all (fun d => is_u64 d) tn ->
+  (cfn,[::i tn]) <- adc n [::i xn] [::i yn] cf0 ->
+  (cfsn, tsn)    <- adc   1     xsn           ysn           cfn ->
+  [:i tsn & tn]  <- adc_v (S n) [:i xsn & xn] [:i ysn & yn] cf0.
+Proof.
+move=> Hlen1 Hlen2 Hlen3 Hall1 Hall2 Hall3 L0 L1.
+move: (combine_chainN_cf Hlen1 Hlen2 Hall1 Hall2 L0 L1) => H.
+move: L0 L1.
+rewrite !ds2i_cons. rewrite Hlen3 Hlen2 Hlen1.
+move/assgnS => [] L0 L1. move/assgnS => [] L2 L3.
+rewrite L1 L3 L0 /adc_v /oflow /Assgn. simp.
+apply Zeq_eq0.
+ring_simplify. rewrite !Nat2Z.inj_succ !Z.pow_succ_r; last apply Zle_0_nat.
+rewrite !ds2i_cons Hlen1 Hlen2 in H. rewrite -H. move: L2; rewrite L0 => L2.
+rewrite -L2.
+ring.
+Qed.
+
+Lemma combine_chainN (n : nat) (xn yn tn : seq Z) (xsn ysn tsn : Z) (cf0 cfn cfsn :bool) :
+  length xn = n ->
+  length yn = n ->
+  length tn = n -> 
+  all (fun d => is_u64 d) xn ->
+  all (fun d => is_u64 d) yn ->
+  all (fun d => is_u64 d) tn ->
+  (cfn,[::i tn])        <- adc n [::i xn] [::i yn] cf0 ->
+  (cfsn,tsn)            <- adc 1     xsn           ysn           cfn ->
+  (cfsn, [:i tsn & tn]) <- adc (S n) [:i xsn & xn] [:i ysn & yn] cf0.
+Proof.
+move=> Hlen1 Hlen2 Hlen3 Hall1 Hall2 Hall3 H1 H2. congr pair.
++ by apply (combine_chainN_cf Hlen1 Hlen2 Hall1 Hall2 H1 H2).
++ by apply (combine_chainN_v Hlen1 Hlen2 Hlen3 Hall1 Hall2 Hall3 H1 H2).
+Qed.
+
+(* ** Ltac for automatic application of combination lemmas *)
+
+Ltac add_len N Tn Xn Yn G1 G2 G3 G4 G5 G6 :=
+  have G1 : (length Xn = N); first done;
+  have G2 : (length Yn = N); first done;
+  have G3 : (length Tn = N); first done;
+  have G4 : all (fun d => is_u64 d) Xn; first band_auto;
+  have G5 : all (fun d => is_u64 d) Yn; first band_auto;
+  have G6 : all (fun d => is_u64 d) Tn; first band_auto.
+
+Ltac combine := (* repeat *)
+  match goal with
+  | [ H1  : (?cf1,_) <- adc 1 ?X0 ?Y0 false,
+      H2  : (_,_)    <- adc 1 ?X1 ?Y1 ?cf1,
+      Bx0 : is_true (is_u64 ?X0),
+      Bx1 : is_true (is_u64 ?X1),
+      By0 : is_true (is_u64 ?Y0),
+      By1 : is_true (is_u64 ?Y1)
+      |- _ ] =>
+    move: (combine_chain1 Bx0 Bx1 By0 By1 H1 H2) => {H1} {H2} H1
+  | [ H1  : (?cf1,ds2i ?Tn) <- adc ?N (ds2i ?Xn)  (ds2i ?Yn) false,
+      H2  : (_,_)           <- adc 1  ?Xsn        ?Ysn       ?cf1
+      |- _ ] =>
+    let Hlen_x := fresh "Hl_x" in
+    let Hlen_y := fresh "Hl_y" in
+    let Hlen_t := fresh "Hl_t" in
+    let Hall_x := fresh "Ha_x" in
+    let Hall_y := fresh "Ha_y" in
+    let Hall_t := fresh "Ha_t" in
+    add_len N Tn Xn Yn Hlen_x Hlen_y Hlen_t Hall_x Hall_y Hall_t;
+    move: (combine_chainN Hlen_x Hlen_y Hlen_t Hall_x Hall_y Hall_t H1 H2)
+      => {H1} {H2} {Hlen_x} {Hlen_y} {Hlen_t} {Hall_x} {Hall_y} {Hall_t} H1
+  end.
+
+(* ** Lemmas for splitting *)
+
+Lemma split_chain1 (x0 y0 x1 y1 t0 t1 : Z) (cf0 cf2 :bool)
+  (B_x0: is_u64 x0)
+  (B_x1: is_u64 x1)
+  (B_y0: is_u64 y0)
+  (B_y1: is_u64 y1) : 
+  (cf2,[:i t1; t0]) <- adc 2 [:i x1; x0] [:i y1; y0] cf0 ->
+  exists cf1,
+    (cf1,t0) <- adc 1 x0 y0 cf0 /\
+    (cf2,t1) <- adc 1 x1 y1 cf1.
+Proof.
+move=> H1. rewrite /adc_v /oflow in H1.
+move : (assgnKl H1) => H2. rewrite -H2 in H1.
+move : (assgnKr H1) => H3. clear H1.
+exists (adc_cf 1 x0 y0 cf0).
+rewrite /adc_v. split.
++ rewrite /Assgn /oflow. congr pair. admit.
++ 
++ rewrite /Assgn. (* done. done. case. move=> [] G1 G2. *)
 Admitted.
 
-(* ** Addition for 4 limbs *)
-
-Definition add_4limb(x0 x1 x2 x3 y0 y1 y2 y3 : Z_w) : (Z_w * Z_w * Z_w * Z_w) := 
-  let (cf, z0) := add  x0 y0      in
-  let (cf, z1) := addc x1 y1 cf   in
-  let (cf, z2) := addc x2 y2 cf   in
-  let (cf, z3) := addc x3 y3 cf   in
-  let u        := cmul cf rem_p64 in
-  let (cf, z0) := add  z0 u       in
-  let (cf, z1) := addc z1 z64 cf  in
-  let (cf, z2) := addc z2 z64 cf  in
-  let (cf, z3) := addc z3 z64 cf  in
-  let add0     := cmul cf rem_p64 in
-  let z0       := add_ncf z0 add0 in
-  (z0,z1,z2,z3).
-
-Lemma corr_add_4_limbs (x0 x1 x2 x3 y0 y1 y2 y3 : Z_w):
-  rem_p = R*R*R*R ->
-  let r := add_4limb x0 x1 x2 x3 y0 y1 y2 y3 in
-  let: (z0,z1,z2,z3) := r in
-        (of64 z0) + (of64 z1)*R + (of64 z2)*R*R + (of64 z3)*R*R*R
-     - ((of64 x0) + (of64 x1)*R + (of64 x2)*R*R + (of64 x3)*R*R*R +
-        (of64 y0) + (of64 y1)*R + (of64 y2)*R*R + (of64 y3)*R*R*R)
-     = 0.
+Lemma split_chainN (n : nat) (xn yn tn : seq Z) (xsn ysn tsn : Z) (cf0 cfsn :bool) :
+  length xn = n ->
+  length yn = n ->
+  length tn = n -> 
+  all (fun d => is_u64 d) xn ->
+  all (fun d => is_u64 d) yn ->
+  all (fun d => is_u64 d) tn ->
+  (cfsn, [:i tsn & tn]) <- adc (S n) [:i xsn & xn] [:i ysn & yn] cf0 ->
+  exists cfn,
+    (cfn,[::i tn]) <- adc n [::i xn] [::i yn] cf0 /\
+    (cfsn,tsn)     <- adc 1 xsn ysn cfn.
 Proof.
-  move=> rem_p_R.
-  rewrite /=.
-  rewrite !(of64_addc_r, of64_addc_ncf, of640, of64_cmul, rem_p_R) /=.
-  ring.
-  (* as in the previous case, we still have to prove absence of overflows *)
-  admit.
 Admitted.
+
+(* ** Addition for 4 limbs  *)
+
+Lemma corr_add_4limb
+  (x0 x1 x2 x3 : Z)
+  (y0 y1 y2 y3 : Z)
+  (t0 t1 t2 t3 : Z)
+  (add1 add2 : Z)
+  (v0 : Z)
+  (z0 z1 z2 z3 : Z)
+  (cf0 cf1 cf2 cf3 : bool)
+  (ccf0 ccf1 ccf2 ccf3 : bool)
+  (cf_f   : bool)
+
+  (B_x0   : is_u64 x0)
+  (B_x1   : is_u64 x1)
+  (B_x2   : is_u64 x2)
+  (B_x3   : is_u64 x3)
+  (B_y0   : is_u64 y0)
+  (B_y1   : is_u64 y1)
+  (B_y2   : is_u64 y2)
+  (B_y3   : is_u64 y3)
+  (B_t0   : is_u64 t0)
+  (B_t1   : is_u64 t1)
+  (B_t2   : is_u64 t2)
+  (B_t3   : is_u64 t3)
+  (B_add1 : is_u64 add1)
+  (B_add2 : is_u64 add2)
+  (B_v0   : is_u64 v0)
+  (B_z0   : is_u64 z0)
+  (B_z1   : is_u64 z1)
+  (B_z2   : is_u64 z2)
+  (B_z3   : is_u64 z3)
+  (B_0    : is_u64 0)
+  (B_38   : is_u64 38) (* FIXME: we should derive bound-facts on constants automatically *)
+  :
+  (cf0,t0)   <- adc 1 x0 y0 false ->
+  (cf1,t1)   <- adc 1 x1 y1 cf0   ->
+  (cf2,t2)   <- adc 1 x2 y2 cf1   -> 
+  (cf3,t3)   <- adc 1 x3 y3 cf2   ->
+  (add1      <- if cf3 then 38 else 0)  ->
+  (ccf0,v0) <- adc 1 t0 add1 false     ->
+  (ccf1,z1) <- adc 1 t1 0    ccf0      ->
+  (ccf2,z2) <- adc 1 t2 0    ccf1      -> 
+  (ccf3,z3) <- adc 1 t3 0    ccf2      ->
+  (add2     <- if ccf3 then 38 else 0)  ->
+  (cf_f,z0) <- adc 1 v0 add2 false
+  ->
+    ds2i [:: z3; z2; z1; z0]
+  = ds2i [:: x3; x2; x1; x0] +
+    ds2i [:: y3; y2; y1; y0] +
+    (cf3:%Z + ccf3:%Z)*(38 - p256).
+Proof.
+(* combine carry chains *)
+pop_defs. repeat combine. sort_defs.
+push_defs. case cf3; last first.
++ pop_defs. simp.
+  rewrite (assgnKr L2).
+  rewrite (assgnKr L0) /adc_v /oflow.
+  rewrite -(assgnKl L0).
+  simp. ring.
++ simp. case ccf3; last first.
+  + pop_defs. simp.
+    rewrite (assgnKr L2) /adc_v /oflow -(assgnKl L2). simp.
+    rewrite (assgnKr L0) /adc_v /oflow -(assgnKl L0). simp.
+    apply Zeq_eq0. ring_simplify. rewrite //=. ring.
+  + pop_defs. simp.
+    rewrite /adc_v /oflow in L4.
+    move : (assgnKl L4) => Heq. rewrite -Heq in L4. simp.
+    have Heq2: cf_f <- false; last first. simp.
+    + rewrite (assgnKr L0) /adc_v in L2.
+      rewrite (assgnKr L4).
+      rewrite (_ : [:i z3; z2; z1; v0 + 38] = [:i z3; z2; z1; v0] + 38); last first.
+      + by rewrite !ds2i_cons Z.pow_0_r; unfold length; ring.
+      rewrite (assgnKr L2).
+      apply Zeq_eq0. simp. ring_simplify.
+      move: (assgnKl L2).
+      rewrite /oflow -(assgnKl L0). simp.
+      move=> <-. unfold ds2i. unfold length. simp. rewrite (_ : 4 = Z.of_nat 4); last done.
+      ring.
+    + move: (@split_chainN 3%nat [:: t2; t1; t0] [:: 0; 0; 38] [:: z2; z1; v0] t3 0 z3 false true).
+      case; try (rewrite //=; fail). band_auto. band_auto. band_auto.
+      move=> cccf2 [] L5 L6.
+
+      move: (@split_chainN 2%nat [:: t1; t0] [:: 0; 38] [:: z1; v0] t2 0 z2 false cccf2).
+      case; try (rewrite //=; fail). band_auto. band_auto. band_auto.
+      move=> cccf1 [] L7 L8.
+
+      move: (@split_chainN 1%nat [:: t0] [:: 38] [:: v0] t1 0 z1 false cccf1).
+      case; try (rewrite //=; fail). band_auto. band_auto. band_auto.
+      move=> cccf0 [] L9 L10.
+      unfold ds2i in L9. unfold length in L9. rewrite !Z.pow_0_r !Z.mul_1_l !Z.add_0_r in L9.
+      push_defs.
+      case cccf0; last (pop_defs; simp; done).
+      case cccf1; last (pop_defs; simp; done).
+      case cccf2; last (pop_defs; simp; done).
+      pop_defs. rewrite (assgnKr L10) in Heq.
+      rewrite /adc_v /oflow in Heq. simp. rewrite -(assgnKl L10) in Heq.
+      simp. rewrite /adc_cf in Heq. move: Heq. case cf_f; last done.
+      move=> G. trans_cmp_b. simp.
+      have: p64 > t0 + 38 - p64 + 38; last done.
+      rewrite (_ : t0 + 38 - p64 + 38 = (t0 - p64) + (38 + 38)); last ring.
+      apply (Zgt_trans _ (0 + (38 + 38))).
+      apply Z.lt_gt; rewrite -Z.ltb_lt; rewrite -lock //=; done.
+      apply Z.lt_gt.
+      apply (Z.add_lt_le_mono); first last. apply Z.eq_le_incl. done.
+      rewrite (Z.lt_sub_0). move: B_t0. rewrite is_u64K. case. done.
+Qed.
